deriving a new key preserves the invariant ms_conn_invariant (easiest case : )

src/tls/ConnInvariant.fst
@@ -36,7 +36,7 @@ let ms_conn_invariant (ms:ms_tab)
 	            (match MM.sel ms (i,r) with 
 		     | None -> True
 		     | Some w -> 
-		       (* Mr.m_sel h (StreamAE.ilog (StreamAE.State.log w)) = Seq.createEmpty)     //we don't even have a connection yet *)
+		       Map.contains h (StreamAE.State.region w) /\
 		       (match Mm.sel conn (idNonce i) with
 		        | None -> Mr.m_sel h (StreamAE.ilog (StreamAE.State.log w)) = Seq.createEmpty     //we don't even have a connection yet
 		       	| Some c -> (exists e. SeqProperties.mem e  (Hh.sel h (HS.log c.hs)) /\ e.w == w)       //registered; NB: CHEAT! We will add a sum between the two kinds of state; a module Epoch with type StAE = StatefulLHAE | StreamAE
@@ -47,14 +47,12 @@ let mc_inv (h:HyperHeap.t) = ms_conn_invariant (Mr.m_sel h Ms.ms_tab) (Mr.m_sel 
 
 //Checking the stability of the invariant
 
-//1. Adding a new log to the ms table (because we tried a lookup at id and it failed)
-//   Easy: because a new log is empty and the id is not in the table already
-//         so, we're in the second case
-//   //3. No connection yet
+//1. Deriving a new key involves adding a new writer to the ms table (because we tried a lookup at id and it failed)
+//   Easy: because a new log is empty and both cases of the conn table allow empty logs to be in ms
 
-
-val add_new_writer: h0:HyperHeap.t -> h1:HyperHeap.t -> i:id -> r:Hh.rid -> w:Ms.writer (i,r) 
+val ms_derive_is_ok: h0:HyperHeap.t -> h1:HyperHeap.t -> i:id -> r:Hh.rid -> w:Ms.writer (i,r) 
   -> Lemma (requires 
+		 Map.contains h1 (StreamAE.State.region w) /\
 		 authId i /\
 		 mc_inv h0 /\ //we're initially in the invariant
 		 Hh.modifies (Set.singleton tls_region) h0 h1 /\ //we just changed the tls_region
@@ -65,54 +63,7 @@ val add_new_writer: h0:HyperHeap.t -> h1:HyperHeap.t -> i:id -> r:Hh.rid -> w:Ms
 		  new_ms = Mm.upd old_ms (i,r) w) /\                                    //and it only changed by adding w
 		 Mr.m_sel h1 (StreamAE.ilog (StreamAE.State.log w)) = Seq.createEmpty)             //and w's log is empty
 	 (ensures mc_inv h1)                                                       //we're back in the invariant
-
-
-assume val gcut: f:(unit -> GTot Type){f()} -> Tot unit
-assume val gadmit: f:(unit -> GTot Type) -> Tot (u:unit{f()})
-
-
-let add_new_writer h0 h1 i r w =  
-  assume (Map.contains h0 tls_region);
-  assume (Hh.contains_ref (Mr.as_rref Ms.ms_tab) h0);
-  assume (Hh.contains_ref (Mr.as_rref conn_table) h0);
-  let old_ms   = Mr.m_sel h0 Ms.ms_tab in
-  let new_ms   = Mr.m_sel h1 Ms.ms_tab in
-  assume (forall j r. 
-	    let wopt = Mm.sel old_ms (j, r) in
-	    is_Some wopt ==>
-	    Hh.disjoint r tls_region 
-	    /\ Map.contains h0 (StreamAE.State.region (Some.v wopt)));
-  ()
-
-
-  (* let j  : id = magic () in  *)
-  (* assume (authId j); *)
-  (* let r' : Hh.rid = magic () in  *)
-  (* match Mm.sel old_ms (j, r') with  *)
-  (*   | None -> admit() *)
-  (*   | Some w' ->  *)
-  (*     (\* assert (Hh.disjoint r' tls_region); *\) *)
-  (*     (\* assert (Hh.disjoint (StreamAE.State.region w') tls_region); *\) *)
-  (*     (\* assume (Map.contains h0 (StreamAE.State.region w')); *\) *)
-  (*     assert (Mr.m_sel h1 (StreamAE.ilog (StreamAE.State.log w')) = Seq.createEmpty); *)
-  (*     admit() *)
-
-
-
-    
-  assert (ms_conn_invariant old_ms new_conn h1);
-  admit()
-  
-  
-  
-  admit()
-
-
-  = admit()
-		 
-		    
-		    	
-
+let ms_derive_is_ok h0 h1 i r w =  ()
 
 //2. Adding a new epoch to a connection c, with a fresh index (hdId i) for c
 //      -- we found a writer w at (ms i), pre-allocated (we're second) or not (we're first)
